proof/TypeClosedSimp.v
@@ -5,6 +5,7 @@ From Coq Require Import Lists.List.
 From Coq Require Import Strings.String.
 From Coq Require Import Logic.FunctionalExtensionality.
 From Coq Require Import Logic.ClassicalFacts.
+From Coq Require Import Logic.Classical.
 From PLF Require Import NormalTypeSystemSimp.
 From PLF Require Import RfTypeDef.
 From PLF Require Import LinearContext.
@@ -26,7 +27,9 @@ Qed.
 Global Hint Resolve state_order_trans: core.
 
 
-Definition closed_refinement_under_state (st: state) (phi: refinement): Prop := forall st', st <st< st' -> phi st = phi st'.
+Definition closed_refinement_under_state (st: state) (phi: refinement): Prop :=
+  forall x, st x = None -> ~ appear_free_in_refinement x phi.
+  (* forall st', st <st< st' -> phi st = phi st'. *)
 
 Global Hint Unfold closed_refinement_under_state: core.
 
@@ -39,97 +42,213 @@ Qed.
 
 Global Hint Resolve empstate_min: core.
 
-Lemma state_order_implies_closed: forall st st' phi,
-    st <st< st' -> closed_refinement_under_state st phi -> closed_refinement_under_state st' phi.
+(* Lemma state_order_implies_closed: forall st st' phi, *)
+(*     st <st< st' -> closed_refinement_under_state st phi -> closed_refinement_under_state st' phi. *)
+(* Proof with eauto. *)
+(*   unfold closed_refinement_under_state. intros. rewrite <- H0... *)
+(* Qed. *)
+
+(* Global Hint Resolve state_order_implies_closed: core. *)
+
+Lemma ZNNPP : forall p:Prop, ~ ~ p <-> p.
 Proof with eauto.
-  unfold closed_refinement_under_state. intros. rewrite <- H0...
+  split. intros. apply NNPP...
+  intros. intros HH. apply HH...
 Qed.
 
-Global Hint Resolve state_order_implies_closed: core.
+Lemma not_appear_free_in_refinement_alt (name: string) (phi: refinement):
+  ~ appear_free_in_refinement name phi <-> (forall st c1, phi st = phi (update st name c1)).
+Proof with eauto.
+  unfold appear_free_in_refinement. rewrite ZNNPP... reflexivity...
+Qed.
 
 Lemma constant_refinement_is_closed: forall (c: constant) (phi: refinement),
     (forall st : state, phi st = (fun c' => c = c')) -> (closed_refinement_under_state empstate phi).
 Proof.
   intros.
-  intros st HH. rewrite H. rewrite H. auto.
+  intros st HH. rewrite not_appear_free_in_refinement_alt. intros. rewrite H. rewrite H. auto.
 Qed.
 
 Lemma refinement_subst_c_closed_rf: forall x1 c2 phi,
-    closed_refinement_under_state empstate phi -> refinement_subst_c x1 c2 phi = phi.
+    closed_refinement_under_state empstate phi -> phi = refinement_subst_c x1 c2 phi.
 Proof with eauto.
   intros.
-  unfold closed_refinement_under_state in H. unfold refinement_subst_c.
-  apply functional_extensionality. intros st.
-  rewrite <- H...
+  assert (forall x, ~ appear_free_in_refinement x phi)... setoid_rewrite not_appear_free_in_refinement_alt in H0.
+  unfold refinement_subst_c.
+  apply functional_extensionality. intros st. rewrite <- H0...
 Qed.
 
 (* closed_type *)
 
-Definition phi_sat_tyst (phi: refinement) (tyst: tystate) (c: constant) :=
-  (forall st, st \TYSTin tyst -> closed_refinement_under_state st phi /\ phi st c).
+(* Definition phi_sat_tyst (phi: refinement) (tyst: tystate) (c: constant) := *)
+(*   (forall st, st \TYSTin tyst -> closed_refinement_under_state st phi /\ phi st c). *)
+
+Definition phi_sat_tyst (phi: refinement) (tyst: tystate) :=
+  (forall x, tyst x = None -> ~ appear_free_in_refinement x phi).
+  (* (forall st, st \TYSTin tyst -> closed_refinement_under_state st phi /\ phi st c). *)
 
 (* Global Hint Unfold nst_tmR_aux: core. *)
 
 Definition lcontxt := linear_context overunderty.
 
-Inductive closed_refinement_in_ctx : tystate -> lcontxt -> refinement -> Prop :=
-| closed_refinement_in_ctx_nil:
-  forall tyst phi, (forall st, st \TYSTin tyst -> closed_refinement_under_state st phi) ->
-              closed_refinement_in_ctx tyst [] phi
-| closed_refinement_in_ctx_overcons: forall tyst x T phix Gamma phi,
-    closed_refinement_in_ctx (update tyst x T) Gamma phi ->
-    closed_refinement_in_ctx tyst ((x, Oty ({{v:T | phix}})) :: Gamma) phi
-| closed_refinement_in_ctx_undercons: forall tyst x T phix Gamma phi,
-    closed_refinement_in_ctx (update tyst x T) Gamma phi ->
-    closed_refinement_in_ctx tyst ((x, Uty ([[v:T | phix]])) :: Gamma) phi
-| closed_refinement_in_ctx_oarrcons: forall tyst x a Ta phia taub Gamma phi,
-    well_formed_type (a o: ({{v:Ta | phia}}) o--> taub) ->
-    closed_refinement_in_ctx tyst Gamma phi ->
-    closed_refinement_in_ctx tyst ((x, Uty (a o: ({{v:Ta | phia}}) o--> taub)) :: Gamma) phi
-| closed_refinement_in_ctx_arrarrcons: forall tyst x t1 t2 Gamma phi,
-    well_formed_type (t1 u--> t2) ->
-    closed_refinement_in_ctx tyst Gamma phi ->
-    closed_refinement_in_ctx tyst ((x, Uty (t1 u--> t2)) :: Gamma) phi.
+Inductive st_type_closed : tystate -> overunderty -> Prop :=
+| st_type_closed_base1: forall tyst (T: base_ty) phi,
+    phi_sat_tyst phi tyst -> st_type_closed tyst ({{v: T | phi}})
+| st_type_closed_base2: forall tyst (T: base_ty) phi,
+    phi_sat_tyst phi tyst -> st_type_closed tyst ([[v: T | phi]])
+| st_type_closed_oarr: forall st x T phi (tau: underty),
+    well_formed_type (x o: ({{v: T | phi}}) o--> tau) ->
+    st x = None ->
+    st_type_closed st ({{v: T | phi}}) ->
+    st_type_closed (x |-> T; st) tau ->
+    st_type_closed st (x o: ({{v: T | phi}}) o--> tau)
+| st_type_closed_arrarr: forall st (tau_x: underty) (tau: underty),
+    well_formed_type (tau_x u--> tau) ->
+    st_type_closed st tau_x ->
+    st_type_closed st tau ->
+    st_type_closed st (tau_x u--> tau).
 
-Global Hint Constructors closed_refinement_in_ctx: core.
+Global Hint Constructors st_type_closed: core.
 
-Lemma closed_refinement_in_ctx_weakening: forall st Gamma1 Gamma2 Gamma3 phi,
-    (Gamma1 ++ Gamma2) = Gamma3 ->
-    closed_refinement_in_ctx st Gamma2 phi ->
-    closed_refinement_in_ctx st Gamma3 phi.
-Admitted.
-
-(* Definition closed_refinement_in_ctx_drop: forall st nst x T phi phi0 e_x, *)
-(*     closed_refinement_in_ctx (st\_ nst _/) [(x, Uty ([[v:T | phi]]))] phi0 -> *)
-(*     empty \N- e_x \Tin T -> *)
-(*     st \NSTin (x |-> (e_x, T); nst) -> *)
-(*     closed_refinement_under_state st phi0. *)
-(* Proof with eauto. *)
-(*   intros st nst x T phi phi0 e_x Hctx HT Hsub. *)
-(*   inversion Hctx; subst... inversion H5;subst... *)
-(* Qed. *)
-
-Lemma closed_refinement_in_ctx_one_underbase: forall tyst x T phi phi0,
-    closed_refinement_in_ctx tyst ((x, Uty ([[v:T | phi]]))::nil) phi0 ->
-    closed_refinement_in_ctx (x |-> T; tyst) [] phi0.
-Admitted.
-
-Global Hint Resolve closed_refinement_in_ctx_one_underbase: core.
-
-Lemma closed_refinement_in_ctx_one_overbase: forall tyst x T phi phi0,
-    closed_refinement_in_ctx tyst ((x, Oty ({{v:T | phi}}))::nil) phi0 ->
-    closed_refinement_in_ctx (x |-> T; tyst) [] phi0.
-Admitted.
-
-Global Hint Resolve closed_refinement_in_ctx_one_overbase: core.
-
-Lemma closed_refinement_in_ctx_destruct_front : forall Gamma tyst x T phi tau,
-    closed_refinement_in_ctx tyst ((x, Uty ([[v:T | phi]])) :: Gamma) tau ->
-    closed_refinement_in_ctx (x |-> T; tyst) Gamma tau.
+Lemma st_type_closed_implies_well_formed_type:
+  forall tyst tau, st_type_closed tyst tau -> well_formed_type tau.
 Proof with eauto.
-  intros Gamma tyst x T phi tau Hclosed.
-  inversion Hclosed; subst...
+  intros.
+  induction H...
 Qed.
+
+Global Hint Resolve st_type_closed_implies_well_formed_type: core.
+
+Fixpoint st_type_closed_in_ctx (tyst: tystate) (Gamma: lcontxt) (tau: overunderty) : Prop :=
+  (match Gamma with
+   | nil => st_type_closed tyst tau
+   | (x, Oty ({{v:T | _}})) :: Gamma | (x, Uty ([[v:T | _]])) :: Gamma =>
+       (* tyst x = None /\ st_type_closed_in_ctx (update tyst x T) Gamma tau *)
+                                        st_type_closed_in_ctx (update tyst x T) Gamma tau
+   | (x, _) :: Gamma => st_type_closed_in_ctx tyst Gamma tau
+   end)
+  /\ well_formed_type tau /\ type_ctx_no_dup tyst Gamma.
+
+(* Inductive st_type_closed_in_ctx : tystate -> lcontxt -> overunderty -> Prop := *)
+(* | st_type_closed_in_ctx_nil: forall tyst tau, st_type_closed tyst tau -> st_type_closed_in_ctx tyst [] tau *)
+(* | st_type_closed_in_ctx_overcons: forall tyst x T phix Gamma tau, *)
+(*     tyst x = None -> *)
+(*     st_type_closed_in_ctx (update tyst x T) Gamma tau -> *)
+(*     type_ctx_no_dup tyst ((x, Oty ({{v:T | phix}})) :: Gamma) -> *)
+(*     st_type_closed_in_ctx tyst ((x, Oty ({{v:T | phix}})) :: Gamma) tau *)
+(* | st_type_closed_in_ctx_undercons: forall tyst x T phix Gamma tau, *)
+(*     tyst x = None -> *)
+(*     st_type_closed_in_ctx (update tyst x T) Gamma tau -> *)
+(*     type_ctx_no_dup tyst (((x, Uty ([[v:T | phix]])) :: Gamma)) -> *)
+(*     st_type_closed_in_ctx tyst ((x, Uty ([[v:T | phix]])) :: Gamma) tau *)
+(* | st_type_closed_in_ctx_oarrcons: forall tyst x a Ta phia taub Gamma tau, *)
+(*     tyst x = None -> *)
+(*     well_formed_type (a o: ({{v:Ta | phia}}) o--> taub) -> *)
+(*     st_type_closed_in_ctx tyst Gamma tau -> *)
+(*     type_ctx_no_dup tyst ((x, Uty (a o: ({{v:Ta | phia}}) o--> taub)) :: Gamma) -> *)
+(*     st_type_closed_in_ctx tyst ((x, Uty (a o: ({{v:Ta | phia}}) o--> taub)) :: Gamma) tau *)
+(* | st_type_closed_in_ctx_arrarrcons: forall tyst x t1 t2 Gamma tau, *)
+(*     tyst x = None -> *)
+(*     well_formed_type (t1 u--> t2) -> *)
+(*     st_type_closed_in_ctx tyst Gamma tau -> *)
+(*     type_ctx_no_dup tyst ((x, Uty (t1 u--> t2)) :: Gamma) -> *)
+(*     st_type_closed_in_ctx tyst ((x, Uty (t1 u--> t2)) :: Gamma) tau. *)
+
+(* Global Hint Constructors st_type_closed_in_ctx: core. *)
+
+
+(* Inductive st_type_closed_in_ctx : tystate -> lcontxt -> refinement -> Prop := *)
+(* | st_type_closed_in_ctx_nil: *)
+(*   forall tyst phi, phi_sat_tyst phi tyst -> st_type_closed_in_ctx tyst [] phi *)
+(*   (* forall tyst phi, (forall st, st \TYSTin tyst -> closed_refinement_under_state st phi) -> *) *)
+(*   (*             st_type_closed_in_ctx tyst [] phi *) *)
+(* | st_type_closed_in_ctx_overcons: forall tyst x T phix Gamma phi, *)
+(*     tyst x = None -> *)
+(*     st_type_closed_in_ctx (update tyst x T) Gamma phi -> *)
+(*     st_type_closed_in_ctx tyst ((x, Oty ({{v:T | phix}})) :: Gamma) phi *)
+(* | st_type_closed_in_ctx_undercons: forall tyst x T phix Gamma phi, *)
+(*     tyst x = None -> *)
+(*     st_type_closed_in_ctx (update tyst x T) Gamma phi -> *)
+(*     st_type_closed_in_ctx tyst ((x, Uty ([[v:T | phix]])) :: Gamma) phi *)
+(* | st_type_closed_in_ctx_oarrcons: forall tyst x a Ta phia taub Gamma phi, *)
+(*     tyst x = None -> *)
+(*     well_formed_type (a o: ({{v:Ta | phia}}) o--> taub) -> *)
+(*     st_type_closed_in_ctx tyst Gamma phi -> *)
+(*     st_type_closed_in_ctx tyst ((x, Uty (a o: ({{v:Ta | phia}}) o--> taub)) :: Gamma) phi *)
+(* | st_type_closed_in_ctx_arrarrcons: forall tyst x t1 t2 Gamma phi, *)
+(*     tyst x = None -> *)
+(*     well_formed_type (t1 u--> t2) -> *)
+(*     st_type_closed_in_ctx tyst Gamma phi -> *)
+(*     st_type_closed_in_ctx tyst ((x, Uty (t1 u--> t2)) :: Gamma) phi. *)
+
+(* Global Hint Constructors st_type_closed_in_ctx: core. *)
+
+(* Lemma appear_free_in_refinement_alt (name: string) (phi: refinement): *)
+(*   appear_free_in_refinement name phi <-> (exists st c2, phi st <> phi (update st name c2)). *)
+(* Proof with eauto. *)
+(*   unfold appear_free_in_refinement. *)
+(* Admitted. *)
+
+(* Lemma st_type_closed_in_ctx_spec: forall tyst phi, *)
+(*     (forall st, st \TYSTin tyst -> closed_refinement_under_state st phi) -> *)
+(*     (forall x, (exists T, tyst x = Some T) <-> (appear_free_in_refinement x phi)). *)
+(* Proof with eauto. *)
+(*   unfold closed_refinement_under_state. unfold state_in_tystate. *)
+(*   intros. split. *)
+(*   - intros He. rewrite -> appear_free_in_refinement_alt. *)
+(*  Admitted. *)
+
+(* Lemma st_type_closed_in_ctx_weakening: forall Gamma1 st Gamma2 phi, *)
+(*     st_type_closed_in_ctx st Gamma2 phi -> *)
+(*     st_type_closed_in_ctx st (Gamma1 ++ Gamma2) phi. *)
+(* Proof with eauto. *)
+(*   induction Gamma1; intros st Gamma2 phi H... *)
+(*   rewrite <- app_comm_cons. *)
+(*   destruct a. destruct o. destruct u. *)
+(*   - constructor... apply IHGamma1... *)
+(*   destruct u... constructor... *)
+
+(* Lemma st_type_closed_in_ctx_weakening: forall Gamma1 st Gamma2 Gamma3 phi, *)
+(*     (Gamma1 ++ Gamma2) = Gamma3 -> *)
+(*     st_type_closed_in_ctx st Gamma2 phi -> *)
+(*     st_type_closed_in_ctx st Gamma3 phi. *)
+(* Proof with eauto. *)
+(*   induction Gamma1; intros st Gamma2 Gamma3 phi Hcc H... *)
+(*   - simpl in Hcc; subst... *)
+(*   - destruct Gamma3. apply app_eq_nil in Hcc. destruct Hcc... inversion H0... *)
+(*     rewrite <- app_comm_cons in Hcc. inversion Hcc. *)
+(*     eapply IHGamma1 in H2... *)
+(*     destruct a. destruct p. inversion H1; subst... *)
+(*     destruct o0... *)
+(*     destruct u... constructor... *)
+
+Lemma st_type_closed_in_ctx_destruct_front : forall Gamma tyst x T phi tau,
+    st_type_closed_in_ctx tyst ((x, Uty ([[v:T | phi]])) :: Gamma) tau ->
+    st_type_closed_in_ctx (x |-> T; tyst) Gamma tau.
+Proof with eauto.
+  intros Gamma tyst x T phi tau Hclosed. simpl in Hclosed...
+  destruct Hclosed...
+Qed.
+
+Lemma st_type_closed_in_ctx_one_underbase: forall tyst x T phi phi0,
+    st_type_closed_in_ctx tyst ((x, Uty ([[v:T | phi]]))::nil) phi0 ->
+    st_type_closed_in_ctx (x |-> T; tyst) [] phi0.
+Proof with eauto.
+  intros tyst x T phi tau Hclosed. simpl in Hclosed...
+  destruct Hclosed; subst...
+Qed.
+
+Global Hint Resolve st_type_closed_in_ctx_one_underbase: core.
+
+Lemma st_type_closed_in_ctx_one_overbase: forall tyst x T phi phi0,
+    st_type_closed_in_ctx tyst ((x, Oty ({{v:T | phi}}))::nil) phi0 ->
+    st_type_closed_in_ctx (x |-> T; tyst) [] phi0.
+Proof with eauto.
+  intros tyst x T phi tau Hclosed.  simpl in Hclosed...
+  destruct Hclosed; subst...
+Qed.
+
+Global Hint Resolve st_type_closed_in_ctx_one_overbase: core.
 
 (* Module ExCloseRefinement. *)
 
@@ -144,7 +263,7 @@ Qed.
 (*     unfold closed_refinement_under_state. reflexivity. *)
 (*   Qed. *)
 
-(*   Example refinement_under_nctx: closed_refinement_in_ctx [("x"%string, TBase TNat)] TNat (fun st c => c = st "x"%string). *)
+(*   Example refinement_under_nctx: st_type_closed_in_ctx [("x"%string, TBase TNat)] TNat (fun st c => c = st "x"%string). *)
 (*   Proof. *)
 (*     constructor. intros. *)
 (*     apply nat_value_n_exists in H. destruct H; subst. *)
@@ -153,61 +272,132 @@ Qed.
 
 (* End ExCloseRefinement. *)
 
-Inductive st_type_closed_in_ctx : tystate -> lcontxt -> overunderty -> Prop :=
-| st_type_closed_base1: forall st Gamma (T: base_ty) phi,
-    closed_refinement_in_ctx st Gamma phi -> st_type_closed_in_ctx st Gamma ({{v: T | phi}})
-| st_type_closed_base2: forall st Gamma (T: base_ty) phi,
-    closed_refinement_in_ctx st Gamma phi -> st_type_closed_in_ctx st Gamma ([[v: T | phi]])
-| st_type_closed_oarr: forall st Gamma x T phi (tau: underty),
-    well_formed_type (x o: ({{v: T | phi}}) o--> tau) ->
-    st_type_closed_in_ctx st Gamma ({{v: T | phi}}) ->
-    st_type_closed_in_ctx st ((x, Oty ({{v: T | phi}})) :: Gamma) tau ->
-    st_type_closed_in_ctx st Gamma (x o: ({{v: T | phi}}) o--> tau)
-| st_type_closed_arrarr: forall st Gamma (tau_x: underty) (tau: underty),
-    well_formed_type (tau_x u--> tau) ->
-    st_type_closed_in_ctx st Gamma tau_x ->
-    st_type_closed_in_ctx st Gamma tau ->
-    st_type_closed_in_ctx st Gamma (tau_x u--> tau).
+(* Inductive st_type_closed_in_ctx : tystate -> lcontxt -> overunderty -> Prop := *)
+(* | st_type_closed_base1: forall st Gamma (T: base_ty) phi, *)
+(*     st_type_closed_in_ctx st Gamma phi -> st_type_closed_in_ctx st Gamma ({{v: T | phi}}) *)
+(* | st_type_closed_base2: forall st Gamma (T: base_ty) phi, *)
+(*     st_type_closed_in_ctx st Gamma phi -> st_type_closed_in_ctx st Gamma ([[v: T | phi]]) *)
+(* | st_type_closed_oarr: forall st Gamma x T phi (tau: underty), *)
+(*     well_formed_type (x o: ({{v: T | phi}}) o--> tau) -> *)
+(*     st_type_closed_in_ctx st Gamma ({{v: T | phi}}) -> *)
+(*     st_type_closed_in_ctx st ((x, Oty ({{v: T | phi}})) :: Gamma) tau -> *)
+(*     st_type_closed_in_ctx st Gamma (x o: ({{v: T | phi}}) o--> tau) *)
+(* | st_type_closed_arrarr: forall st Gamma (tau_x: underty) (tau: underty), *)
+(*     well_formed_type (tau_x u--> tau) -> *)
+(*     st_type_closed_in_ctx st Gamma tau_x -> *)
+(*     st_type_closed_in_ctx st Gamma tau -> *)
+(*     st_type_closed_in_ctx st Gamma (tau_x u--> tau). *)
 
-Global Hint Constructors st_type_closed_in_ctx: core.
+(* Global Hint Constructors st_type_closed_in_ctx: core. *)
 
 Lemma st_type_closed_in_ctx_implies_well_formed_type:
   forall tyst Gamma tau, st_type_closed_in_ctx tyst Gamma tau -> well_formed_type tau.
-Admitted.
+Proof with eauto.
+  intros.
+  destruct Gamma. simpl in H.
+  destruct H. destruct H0...
+  destruct H. destruct H0...
+Qed.
 
 Global Hint Resolve st_type_closed_in_ctx_implies_well_formed_type: core.
 
-Lemma st_type_closed_in_ctx_emp_implies_all_not_free: forall Gamma (tau: underty) x,
-    l_find_right_most Gamma x = None ->
-    st_type_closed_in_ctx empty Gamma tau ->
+Lemma st_type_closed_in_ctx_implies_type_ctx_no_dup: forall st Gamma tau,
+    st_type_closed_in_ctx st Gamma tau -> type_ctx_no_dup st Gamma.
+Proof with eauto.
+  intros.
+  destruct Gamma. simpl in H.
+  destruct H. destruct H0...
+  destruct H. destruct H0...
+Qed.
+
+Global Hint Resolve st_type_closed_in_ctx_implies_type_ctx_no_dup: core.
+
+Lemma st_type_closed_implies_over_not_free: forall x (tau:overbasety),
+    st_type_closed empty tau ->
+    ~ appear_free_in_overbasety x tau.
+Proof with eauto.
+  intros. inversion H; subst. simpl...
+Qed.
+
+Lemma st_type_closed_implies_not_free: forall x (tau:underty) st,
+    st x = None ->
+    st_type_closed st tau ->
     ~ appear_free_in_underty x tau.
-Admitted.
+Proof with eauto.
+  intro x.
+  induction tau; intros st Hst H...
+  - inversion H; subst...
+  - inversion H; subst... simpl. intro HF. destruct HF...
+    + inversion H6; subst. apply H4 in H0...
+    + destruct H0. eapply IHtau in H7... rewrite update_neq...
+  - inversion H; subst... simpl. intro HF. destruct HF...
+    + eapply  IHtau1  in H4...
+    + eapply  IHtau2  in H5...
+Qed.
 
-Global Hint Resolve st_type_closed_in_ctx_emp_implies_all_not_free: core.
+Global Hint Resolve st_type_closed_implies_not_free: core.
 
-Lemma st_type_closed_in_ctx_emp_implies_all: forall st Gamma tau,
-    st_type_closed_in_ctx empty Gamma tau -> st_type_closed_in_ctx st Gamma tau.
-Admitted.
+Lemma st_type_closed_in_ctx_emp_implies_all_not_free: forall x Gamma (tau: underty) st,
+    st x = None ->
+    l_find_right_most Gamma x = None ->
+    st_type_closed_in_ctx st Gamma tau ->
+    ~ appear_free_in_underty x tau.
+Proof with eauto.
+  intro x.
+  induction Gamma; intros tau st Hst Hfind HH...
+  - inversion HH; subst...
+  - destruct a. inversion HH; subst...
+    destruct o. destruct u.
+    + destruct H0. simpl in Hfind.
+      assert (l_find_right_most Gamma x = None). apply l_find_right_most_none_neq_tl in Hfind...
+      eapply IHGamma in H... rewrite update_neq...
+    + assert (l_find_right_most Gamma x = None). apply l_find_right_most_none_neq_tl in Hfind...
+      eapply IHGamma in H1...
+    + assert (l_find_right_most Gamma x = None). apply l_find_right_most_none_neq_tl in Hfind...
+      eapply IHGamma in H1...
+    + destruct o.
+      assert (l_find_right_most Gamma x = None). apply l_find_right_most_none_neq_tl in Hfind...
+      eapply IHGamma in H... rewrite update_neq...
+Qed.
 
-Global Hint Resolve st_type_closed_in_ctx_emp_implies_all: core.
+
+(* Global Hint Resolve st_type_closed_in_ctx_emp_implies_all_not_free: core. *)
+
+(* Lemma st_type_closed_in_ctx_emp_implies_all: forall st Gamma tau, *)
+(*     st_type_closed_in_ctx empty Gamma tau -> st_type_closed_in_ctx st Gamma tau. *)
+(* Admitted. *)
+
+(* Global Hint Resolve st_type_closed_in_ctx_emp_implies_all: core. *)
+
+Lemma st_type_closed_in_ctx_implies_head_unique: forall Gamma st s tau_s tau,
+    st_type_closed_in_ctx st ((s, tau_s) :: Gamma) tau ->
+    l_find_right_most Gamma s = None.
+Proof with eauto.
+  intros...
+Qed.
 
 Lemma st_type_closed_in_ctx_perm: forall tyst a tau_a b tau_b Gamma,
-    st_type_closed_in_ctx tyst [] tau_b ->
+    a <> b ->
     (forall tau, st_type_closed_in_ctx tyst ((a, tau_a)::(b, tau_b)::Gamma) tau ->
             st_type_closed_in_ctx tyst ((b, tau_b)::(a, tau_a)::Gamma) tau).
+Proof with eauto.
+  intros tyst a tau_a b tau_b Gamma Hab. intros.
+  destruct tau_a.
+  destruct u. simpl in H... destruct H... split... destruct H. clear H. clear H0.
+  - destruct tau_b. destruct u.
 Admitted.
 
-Lemma st_type_closed_in_ctx_one_underbase: forall tyst x T phi tau,
-    st_type_closed_in_ctx tyst ((x, Uty ([[v:T | phi]]))::nil) tau ->
-    st_type_closed_in_ctx (x |-> T; tyst) [] tau.
-Admitted.
+(* Lemma st_type_closed_in_ctx_one_underbase: forall tyst x T phi tau, *)
+(*     st_type_closed_in_ctx tyst ((x, Uty ([[v:T | phi]]))::nil) tau -> *)
+(*     st_type_closed_in_ctx (x |-> T; tyst) [] tau. *)
+(* Admitted. *)
 
 Global Hint Resolve st_type_closed_in_ctx_one_underbase: core.
 
-Lemma st_type_closed_in_ctx_one_overbase: forall tyst x T phi tau,
-    st_type_closed_in_ctx tyst ((x, Oty ({{v:T | phi}}))::nil) tau ->
-    st_type_closed_in_ctx (x |-> T; tyst) [] tau.
-Admitted.
+(* Lemma st_type_closed_in_ctx_one_overbase: forall tyst x T phi tau, *)
+(*     st_type_closed_in_ctx tyst ((x, Oty ({{v:T | phi}}))::nil) tau -> *)
+(*     st_type_closed_in_ctx (x |-> T; tyst) [] tau. *)
+(* Admitted. *)
 
 Global Hint Resolve st_type_closed_in_ctx_one_overbase: core.
 
@@ -216,18 +406,16 @@ Lemma st_type_closed_in_ctx_destruct_underbase_front : forall Gamma tyst x T phi
     st_type_closed_in_ctx (x |-> T; tyst) Gamma tau.
 Proof with eauto.
   intros Gamma tyst x T phi tau Hclosed.
-  induction Gamma; inversion Hclosed; subst.
-  + inversion H...
-  + inversion H...
-  + inversion H...
-  + inversion H; subst...
-Admitted.
+  destruct Hclosed...
+Qed.
 
 Lemma st_type_closed_in_ctx_destruct_overbase_front : forall Gamma tyst x T phi tau,
     st_type_closed_in_ctx tyst ((x, Oty ({{v:T | phi}})) :: Gamma) tau ->
     st_type_closed_in_ctx (x |-> T; tyst) Gamma tau.
 Proof with eauto.
-Admitted.
+  intros Gamma tyst x T phi tau Hclosed.
+  destruct Hclosed...
+Qed.
 
 Global Hint Resolve st_type_closed_in_ctx_destruct_overbase_front: core.
 
@@ -235,13 +423,17 @@ Lemma st_type_closed_in_ctx_destruct_arrar_front : forall Gamma tyst x t1 t2 tau
     st_type_closed_in_ctx tyst ((x, Uty (t1 u--> t2)) :: Gamma) tau ->
     st_type_closed_in_ctx tyst Gamma tau.
 Proof with eauto.
-Admitted.
+  intros Gamma tyst x T phi tau Hclosed.
+  destruct Hclosed...
+Qed.
 
 Lemma st_type_closed_in_ctx_destruct_oarr_front : forall Gamma tyst x a Ta phia t2 tau,
     st_type_closed_in_ctx tyst ((x, Uty (a o: {{v:Ta | phia}} o--> t2)) :: Gamma) tau ->
     st_type_closed_in_ctx tyst Gamma tau.
 Proof with eauto.
-Admitted.
+  intros Gamma tyst x a Ta phia t2 tau Hclosed.
+  destruct Hclosed...
+Qed.
 
 (* Inductive overunderbasety : Type := *)
 (* | Obase: base_ty -> refinement -> overunderbasety *)
@@ -268,10 +460,10 @@ Admitted.
 
 (* Inductive type_closed_in_ctx : basecontxt -> overunderty -> Prop := *)
 (* | type_closed_base1: forall Gamma (T: base_ty) phi, *)
-(*     closed_refinement_in_ctx (erase_basetypectx Gamma) T phi -> *)
+(*     st_type_closed_in_ctx (erase_basetypectx Gamma) T phi -> *)
 (*     type_closed_in_ctx Gamma ({{v: T | phi}}) *)
 (* | type_closed_base2: forall Gamma (T: base_ty) phi, *)
-(*     closed_refinement_in_ctx (erase_basetypectx Gamma) T phi -> *)
+(*     st_type_closed_in_ctx (erase_basetypectx Gamma) T phi -> *)
 (*     type_closed_in_ctx Gamma ([[v: T | phi]]) *)
 (* | type_closed_oarr: forall Gamma x T phi (tau: underty), *)
 (*     type_closed_in_ctx Gamma ({{v: T | phi}}) -> *)
@@ -294,35 +486,29 @@ Admitted.
 (*       end *)
 (*   end. *)
 
-Definition type_closed_in_ctx (Gamma: lcontxt) (tau: overunderty):= st_type_closed_in_ctx empty Gamma tau.
-
-Global Hint Unfold type_closed_in_ctx: core.
-
 (* type closed \S{Ty} *)
 
-Lemma mk_op_is_type_closed: forall op a b, type_closed_in_ctx l_empty (mk_op op a b).
+Lemma mk_op_is_type_closed: forall st op a b, st_type_closed_in_ctx st l_empty (mk_op op a b).
 Admitted.
 
 Global Hint Resolve mk_op_is_type_closed: core.
 
-Lemma mk_eq_over_base_is_type_closed: forall x T phi, type_closed_in_ctx ((x, Oty ({{v:T | phi}}))::nil) (mk_eq_var T x).
+Lemma mk_eq_over_base_is_type_closed: forall x T phi, st_type_closed_in_ctx empty ((x, Oty ({{v:T | phi}}))::nil) (mk_eq_var T x).
 Proof with eauto.
   intros x T phi. repeat constructor...
-  unfold closed_refinement_under_state... simpl. intros st Hst st' Hsub.
-  remember (Hst x) as Hst'. clear HeqHst'. rewrite update_eq in Hst'. edestruct Hst'.
-  reflexivity.
-  rewrite H. apply Hsub in H. rewrite H. reflexivity.
+  unfold phi_sat_tyst. intros. intro HH.
+  destruct (eqb_spec x x0); subst... rewrite update_eq in H. inversion H.
+  unfold appear_free_in_refinement in HH. apply HH. intros. rewrite update_neq...
 Qed.
 
 Global Hint Resolve mk_eq_over_base_is_type_closed: core.
 
-Lemma mk_eq_under_base_is_type_closed: forall x T phi, type_closed_in_ctx ((x, Uty ([[v:T | phi]]))::nil) (mk_eq_var T x).
+Lemma mk_eq_under_base_is_type_closed: forall x T phi, st_type_closed_in_ctx empty ((x, Uty ([[v:T | phi]]))::nil) (mk_eq_var T x).
 Proof with eauto.
   intros x T phi. repeat constructor...
-  unfold closed_refinement_under_state... intros st Hst st' Hsub.
-  remember (Hst x) as Hst'. clear HeqHst'. rewrite update_eq in Hst'. edestruct Hst'.
-  reflexivity.
-  rewrite H. apply Hsub in H. rewrite H. reflexivity.
+  unfold phi_sat_tyst. intros. intro HH.
+  destruct (eqb_spec x x0); subst... rewrite update_eq in H. inversion H.
+  unfold appear_free_in_refinement in HH. apply HH. intros. rewrite update_neq...
 Qed.
 
 Global Hint Resolve mk_eq_under_base_is_type_closed: core.
@@ -341,16 +527,47 @@ Proof.
   setoid_rewrite H. auto.
 Qed.
 
-Lemma constant_eq_is_close: forall Gamma c, type_closed_in_ctx Gamma (mk_eq_constant c).
-Proof.
-  intros. constructor.
+Lemma constant_is_wf: forall c, well_formed_type (mk_eq_constant c).
+Proof with eauto.
+  intros.
+  destruct c; constructor...
+Qed.
+
+Global Hint Resolve constant_is_wf: core.
+
+Lemma nodup_update: forall st s b r Gamma,
+    type_ctx_no_dup st ((s, Uty ([[v:b | r]])) :: Gamma) ->
+    type_ctx_no_dup (s |-> b; st) Gamma.
 Admitted.
-(*   assert (closed_refinement_in_ctx nil (ty_of_cotyst c) (fun (_ : state) (v : constant) => v = c)). *)
-(*   constructor. *)
-(*   unfold closed_refinement_under_state; destruct c; simpl; reflexivity. *)
-(*   apply closed_refinement_in_ctx_weakening with (Gamma1 := (erase_basetypectx (lcontxt_to_baseconctx Gamma))) (Gamma2 := nil); auto. *)
-(*   rewrite app_nil_r. auto. *)
-(* Qed. *)
+
+Lemma nodup_update_over: forall st s b r Gamma,
+    type_ctx_no_dup st ((s, Oty ({{v:b | r}})) :: Gamma) ->
+    type_ctx_no_dup (s |-> b; st) Gamma.
+Admitted.
+
+Lemma nodup_dropfst: forall st s tau_s Gamma,
+    type_ctx_no_dup st ((s, tau_s) :: Gamma) ->
+    type_ctx_no_dup st Gamma.
+Proof with eauto.
+  intros. rewrite <- app_one_is_cons in H...
+Qed.
+
+(* Global Hint Resolve nodup_dropfst: core. *)
+
+Lemma constant_eq_is_close: forall Gamma st c,
+    type_ctx_no_dup st Gamma ->
+    st_type_closed_in_ctx st Gamma (mk_eq_constant c).
+Proof with eauto.
+  induction Gamma; intros...
+  - repeat constructor...
+    intros x' Hx'. rewrite not_appear_free_in_refinement_alt. intros...
+  - destruct a.
+    destruct o... destruct u...
+    + constructor... apply IHGamma... eapply nodup_update...
+    + constructor. apply IHGamma. apply nodup_dropfst in H... split...
+    + constructor. apply IHGamma. apply nodup_dropfst in H... split...
+    + destruct o... constructor. apply IHGamma. eapply nodup_update_over... split...
+Qed.
 
 Global Hint Resolve mk_eq_constant_spec: core.
 Global Hint Resolve subst_constant_eq: core.
@@ -358,37 +575,57 @@ Global Hint Resolve constant_eq_is_close: core.
 
 (* type closed lemmas *)
 
-Lemma type_closed_add_post: forall (Gamma1 Gamma2: lcontxt) (tau: overunderty),
-    type_closed_in_ctx Gamma1 tau -> type_closed_in_ctx (Gamma1 ++ Gamma2) tau.
+Lemma mk_eq_is_well_formed_type: forall T x, well_formed_type (mk_eq_var T x).
 Admitted.
 
-Lemma type_closed_add_pre: forall (Gamma1 Gamma2: lcontxt) (tau: overunderty),
-    type_closed_in_ctx Gamma2 tau -> type_closed_in_ctx (Gamma1 ++ Gamma2) tau.
+Global Hint Resolve mk_eq_is_well_formed_type: core.
+
+Lemma type_closed_add_post: forall (Gamma1 Gamma2: lcontxt) st (tau: overunderty),
+    type_ctx_no_dup st (Gamma1 ++ Gamma2) ->
+    st_type_closed_in_ctx st Gamma1 tau -> st_type_closed_in_ctx st (Gamma1 ++ Gamma2) tau.
 Admitted.
 
-Lemma st_type_closed_in_ctx_last_over_var: forall st Gamma x T phi, st (Gamma ++ ((x, Oty ({{v:T | phi}}))::nil)) (mk_eq_var T x).
+Lemma type_closed_add_pre: forall (Gamma1 Gamma2: lcontxt) st (tau: overunderty),
+    type_ctx_no_dup st (Gamma1 ++ Gamma2) ->
+    st_type_closed_in_ctx st Gamma2 tau -> st_type_closed_in_ctx st (Gamma1 ++ Gamma2) tau.
 Admitted.
 
-Lemma st_type_closed_in_ctx_last_under_var: forall st Gamma x T phi, st (Gamma ++ ((x, Uty ([[v:T | phi]]))::nil)) (mk_eq_var T x).
-Admitted.
+Lemma st_type_closed_in_ctx_last_over_var: forall st Gamma x T phi,
+    type_ctx_no_dup st (Gamma ++ ((x, Oty ({{v:T | phi}}))::nil)) ->
+    st_type_closed_in_ctx st (Gamma ++ ((x, Oty ({{v:T | phi}}))::nil)) (mk_eq_var T x).
+Proof with eauto.
+  intros. apply type_closed_add_pre...
+  constructor. constructor... constructor...
+  unfold phi_sat_tyst. intros. intro HH.
+  destruct (eqb_spec x x0); subst... rewrite update_eq in H0. inversion H0.
+  unfold appear_free_in_refinement in HH. apply HH. intros. rewrite update_neq...
+  split; auto. eapply type_ctx_no_dup_ctx_post in H...
+Qed.
 
-Lemma type_closed_drop_post: forall (Gamma1 Gamma2: lcontxt) (tau: overunderty),
-	  (forall x tau_x, l_find_right_most Gamma2 x = Some tau_x -> ~ appear_free_in_overunderty x tau) ->
-	  type_closed_in_ctx (Gamma1 ++ Gamma2) tau -> type_closed_in_ctx Gamma1 tau.
-Admitted.
+Lemma st_type_closed_in_ctx_last_under_var: forall st Gamma x T phi,
+    type_ctx_no_dup st (Gamma ++ ((x, Uty ([[v:T | phi]]))::nil)) ->
+    st_type_closed_in_ctx st (Gamma ++ ((x, Uty ([[v:T | phi]]))::nil)) (mk_eq_var T x).
+Proof with eauto.
+  intros. apply type_closed_add_pre...
+  constructor. constructor... constructor...
+  unfold phi_sat_tyst. intros. intro HH.
+  destruct (eqb_spec x x0); subst... rewrite update_eq in H0. inversion H0.
+  unfold appear_free_in_refinement in HH. apply HH. intros. rewrite update_neq...
+  split; auto. eapply type_ctx_no_dup_ctx_post in H...
+Qed.
 
-Global Hint Resolve type_closed_add_pre: core.
-Global Hint Resolve type_closed_add_post: core.
+(* Global Hint Resolve type_closed_add_pre: core. *)
+(* Global Hint Resolve type_closed_add_post: core. *)
 
-Fixpoint erase_arr_bindings (Gamma: lcontxt): lcontxt :=
-  match Gamma with
-  | nil => nil
-  | (x, ty)::Gamma =>
-      match ty with
-      | Oty _ | Uty ([[v: _ | _ ]]) => (x, ty)::(erase_arr_bindings Gamma)
-      | _ => (erase_arr_bindings Gamma)
-      end
-  end.
+(* Fixpoint erase_arr_bindings (Gamma: lcontxt): lcontxt := *)
+(*   match Gamma with *)
+(*   | nil => nil *)
+(*   | (x, ty)::Gamma => *)
+(*       match ty with *)
+(*       | Oty _ | Uty ([[v: _ | _ ]]) => (x, ty)::(erase_arr_bindings Gamma) *)
+(*       | _ => (erase_arr_bindings Gamma) *)
+(*       end *)
+(*   end. *)
 
 (* Lemma erase_arr_bindings_spec: forall (Gamma: lcontxt), *)
 (*     lcontxt_to_baseconctx Gamma = lcontxt_to_baseconctx (erase_arr_bindings Gamma). *)
@@ -400,10 +637,10 @@ Fixpoint erase_arr_bindings (Gamma: lcontxt): lcontxt :=
 (*   - destruct o. simpl. rewrite IHGamma. auto. *)
 (* Qed. *)
 
-Lemma type_closed_even_without_arr_bindings: forall Gamma tau,
-    type_closed_in_ctx Gamma tau <-> type_closed_in_ctx (erase_arr_bindings Gamma) tau.
-Proof.
-Admitted.
+(* Lemma type_closed_even_without_arr_bindings: forall Gamma tau, *)
+(*     type_closed_in_ctx Gamma tau <-> type_closed_in_ctx (erase_arr_bindings Gamma) tau. *)
+(* Proof. *)
+(* Admitted. *)
 (*   unfold type_closed. setoid_rewrite <- erase_arr_bindings_spec. reflexivity. *)
 (* Qed. *)
 
@@ -495,3 +732,7 @@ Global Hint Resolve st_type_closed_ctx_pre: core.
 (* Lemma st_type_closed_ctx_even_without_arr_bindings: forall st Gamma, *)
 (*     st_type_closed_ctx st Gamma -> st_type_closed_ctx (erase_arr_bindings Gamma). *)
 (* Admitted. *)
+
+Definition type_closed_in_ctx (Gamma: lcontxt) (tau: overunderty):= st_type_closed_in_ctx empty Gamma tau.
+
+Global Hint Unfold type_closed_in_ctx: core.
