proof/TypeDisj.v
@@ -23,6 +23,8 @@ Definition disjunct (Gamma: context) (tau1 tau2 tau3: underty) :=
 
 Notation "Gamma '\C-' tau1 '\tyor' tau2 '\tyeq' tau3 " := (disjunct Gamma tau1 tau2 tau3) (at level 40).
 
-Lemma disj_same_ty: forall Gamma tau1 tau2 tau3,
-  Gamma \C- tau1 \tyor tau2 \tyeq tau3 -> u\_ tau1 _/ =  u\_ tau3 _/ /\ u\_ tau2 _/ =  u\_ tau3 _/.
-Admitted.
+(* Lemma disj_same_ty: forall Gamma tau1 tau2 tau3, *)
+(*   Gamma \C- tau1 \tyor tau2 \tyeq tau3 -> u\_ tau1 _/ =  u\_ tau3 _/ /\ u\_ tau2 _/ =  u\_ tau3 _/. *)
+(* Proof with eauto. *)
+(*   intros. *)
+(*   split. edestruct H. *)
